Finish Zp and BigZp

execution/theories/BoardroomMath.v
@@ -15,7 +15,7 @@ Import ListNotations.
 
 Local Open Scope Z.
 
-Class FField {A : Type} :=
+Class BoardroomField {A : Type} :=
   build_ffield {
     elmeq : A -> A -> Prop;
     elmeq_dec x y : {elmeq x y} + {~(elmeq x y)};
@@ -57,10 +57,6 @@ Class FField {A : Type} :=
 
     opp_inv_l a : elmeq (add (opp a) a) zero;
     inv_inv_l a : ~(elmeq a zero) -> elmeq (mul (inv a) a) one;
-    inv_mul a b :
-      ~(elmeq a zero) ->
-      ~(elmeq b zero) ->
-      inv (mul a b) = mul (inv a) (inv b);
 
     mul_add a b c : elmeq (mul (add a b) c) (add (mul a c) (mul b c));
 
@@ -87,7 +83,7 @@ Class FField {A : Type} :=
       ~(elmeq (inv a) zero);
   }.
 
-Arguments FField : clear implicits.
+Arguments BoardroomField : clear implicits.
 
 Delimit Scope ffield_scope with ffield.
 
@@ -102,7 +98,7 @@ Notation "a 'exp=' b" := (expeq a b) (at level 70) : ffield.
 Notation "a 'exp<>' b" := (~(expeq a b)) (at level 70) : ffield.
 
 Local Open Scope ffield.
-Global Instance oeq_equivalence {A : Type} (field : FField A) : Equivalence expeq.
+Global Instance oeq_equivalence {A : Type} (field : BoardroomField A) : Equivalence expeq.
 Proof.
   unfold expeq.
   constructor.
@@ -111,7 +107,7 @@ Proof.
   - now intros ? ? ? -> ->.
 Qed.
 
-Definition FField_field_theory {A : Type} (field : FField A) :
+Definition BoardroomField_field_theory {A : Type} (field : BoardroomField A) :
   field_theory
     zero one
     add mul
@@ -134,13 +130,13 @@ Proof.
   - apply inv_inv_l.
 Qed.
 
-Class Generator {A : Type} (field : FField A) :=
+Class Generator {A : Type} (field : BoardroomField A) :=
   build_generator {
     generator : A;
     generator_nonzero : generator !== 0;
   }.
 
-Class DiscreteLog {A : Type} (field : FField A) (g : Generator field) :=
+Class DiscreteLog {A : Type} (field : BoardroomField A) (g : Generator field) :=
   build_log {
     (* This is computationally intractable, but we still elmequire it
     for ease of specification *)
@@ -160,13 +156,13 @@ Class DiscreteLog {A : Type} (field : FField A) (g : Generator field) :=
     log_generator : log generator = 1%Z;
   }.
 
-Section WithFField.
+Section WithBoardroomField.
   Context {A : Type}.
-  Context {field : FField A}.
+  Context {field : BoardroomField A}.
   Context {gen : Generator field}.
   Context {disc_log : DiscreteLog field gen}.
 
-  Add Field ff : (FField_field_theory field).
+  Add Field ff : (BoardroomField_field_theory field).
 
   Local Open Scope ffield.
 
@@ -298,7 +294,7 @@ Section WithFField.
     - apply F2AF.
       + typeclasses eauto.
       + constructor; typeclasses eauto.
-      + apply (FField_field_theory field).
+      + apply (BoardroomField_field_theory field).
   Qed.
 
   Hint Resolve int_domain : core.
@@ -689,926 +685,9 @@ Section WithFField.
       rewrite sum_lemma.
       reflexivity.
   Qed.
+End WithBoardroomField.
 
-  (*
-  Lemma Z_eta z : match z with
-                  | Z0 => Z0
-                  | Zpos p => Zpos p
-                  | Zneg p => Zneg p
-                  end = z.
-  Proof. now destruct z. Qed.
-
-  (*
-  Lemma sumZ_firstn_whole (f : Z -> Z) n (l : list Z) :
-    sumZ f (firstn n l) =
-    sumZ (fun i => if Nat.ltb i (length l) then f (nth i l 0%Z) else 0%Z) (seq 0 n).
-  Proof.
-    revert l f.
-    induction n as [|n IH]; intros l f; auto.
-    cbn -[Nat.ltb].
-    rewrite sumZ_seq_n.
-    destruct l as [|hd tl].
-    - cbn.
-      clear.
-      induction (seq 0 n); auto.
-    - cbn -[Nat.ltb].
-      apply f_equal.
-      rewrite IH.
-      apply sumZ_exteq_proper; auto.
-      intro a.
-      replace (a + 1 <? S (length tl))%nat with (a <? length tl)%nat; cycle 1.
-      { destruct (Nat.ltb_spec a (length tl)), (Nat.ltb_spec (a + 1) (S (length tl)));
-          cbn in *; auto; lia. }
-      destruct (Nat.ltb_spec a (length tl)); auto.
-      destruct (a + 1)%nat eqn:a1; try lia.
-      now replace a with n0 by lia.
-  Qed.
-
-  Lemma sumZ_skipn_whole (f : Z -> Z) n (l : list Z) :
-    sumZ f (skipn n l) =
-    sumZ (fun i => if Nat.ltb n i && Nat.ltb i (length l) then f (nth i l 0%Z) else 0%Z) (seq 0 n).
-  Proof.
-    replace (skipn n l) with (rev (firstn (length l - n) (rev l))) by admit.
-    rewrite <- Permutation.Permutation_rev.
-    rewrite sumZ_firstn_whole.
-    induction l as [|x xs IH].
-    - cbn.
-      induction (seq 0 n); cbn; auto.
-      rewrite <- IHl.
-      destruct a; auto.
-      destruct n; auto.
-      cbn.
-    apply sumZ_exteq_proper; auto.
-    intros a.
-    rewrite rev_length.
-    destruct
-    rewrite rev_nth.
-    rewrite sumZ_firstn_whole.
-    revert l f.
-    induction n as [|n IH]; intros l f.
-    - cbn.
-    cbn -[Nat.ltb].
-    rewrite sumZ_seq_n.
-    destruct l as [|hd tl].
-    - cbn.
-      clear.
-      induction (seq 0 n); auto.
-    - cbn -[Nat.ltb].
-      apply f_equal.
-      rewrite IH.
-      apply sumZ_exteq_proper; auto.
-      intro a.
-      replace (a + 1 <? S (length tl))%nat with (a <? length tl)%nat; cycle 1.
-      { destruct (Nat.ltb_spec a (length tl)), (Nat.ltb_spec (a + 1) (S (length tl)));
-          cbn in *; auto; lia. }
-      destruct (Nat.ltb_spec a (length tl)); auto.
-      destruct (a + 1)%nat eqn:a1; try lia.
-      now replace a with n0 by lia.
-
-  Lemma sum_split_center (l : list Z) i :
-    sumZ id (firstn i l) - sumZ id (skipn (S i) l) =
-    sumZ (fun j => (if Nat.ltb j i then 1
-                    else if Nat.eqb j i then 0
-                    else (-1)) * nth j l 0)%Z
-         (seq 0 (length l)).
-  Proof.
-    destruct (i <=? length l)%nat eqn:le; [apply Nat.leb_le in le|apply Nat.leb_gt in le];
-      cycle 1.
-    {
-      rewrite firstn_all2, skipn_none by lia.
-      cbn -[Nat.ltb].
-      rewrite Z.sub_0_r.
-      revert l le.
-      induction i as [|i IH]; intros l le.
-      - lia.
-      - destruct l; auto.
-        cbn in le.
-        specialize (IH l ltac:(lia)).
-        cbn.
-        rewrite sumZ_seq_n.
-        rewrite Z_eta.
-        apply f_equal.
-        rewrite IH.
-        apply sumZ_exteq_proper; auto.
-        clear.
-        intros n.
-        replace (n + 1)%nat with (S n) by lia.
-        repeat
-          match goal with
-          | [|- context[Nat.ltb ?a ?b]] => destruct (Nat.ltb_spec a b)
-          | [|- context[Nat.leb ?a ?b]] => destruct (Nat.leb_spec a b)
-          | [|- context[Nat.eqb ?a ?b]] => destruct (Nat.eqb_spec a b)
-          end;
-          cbn in *; lia.
-    }
-
-    revert l le.
-    induction i as [|i IH]; intros l le.
-    - cbn.
-      induction l as [|x xs IH]; auto.
-      cbn.
-      rewrite sumZ_seq_n.
-      destruct xs; auto.
-      cbn.
-      fold (Z.opp z).
-      unfold id.
-      replace (-(z + sumZ (fun x => x) xs)) with (-z + (- sumZ (fun x => x) xs))%Z by lia.
-      apply f_equal.
-      unfold id in IH; rewrite IH.
-      rewrite (sumZ_seq_n _ 1).
-      rewrite Z_eta.
-    - destruct l; auto.
-      cbn.
-      rewrite Z_eta.
-      unfold id.
-      rewrite <- Z.add_sub_assoc.
-      apply f_equal.
-      rewrite sumZ_seq_n.
-      rewrite IH.
-      apply sumZ_exteq_proper; auto.
-      intros n.
-      replace (n + 1)%nat with (S n) by lia.
-      repeat
-        match goal with
-        | [|- context[Nat.ltb ?a ?b]] => destruct (Nat.ltb_spec a b)
-        | [|- context[Nat.leb ?a ?b]] => destruct (Nat.leb_spec a b)
-        | [|- context[Nat.eqb ?a ?b]] => destruct (Nat.eqb_spec a b)
-        end;
-        cbn in *; lia.
-
-    destruct (i <=? length l)%nat eqn:le; [apply Nat.leb_le in le|apply Nat.leb_gt in le];
-      cycle 1.
-    {
-      rewrite firstn_all2, skipn_none by lia.
-      cbn -[Nat.ltb].
-      rewrite Z.sub_0_r.
-      revert l le.
-      induction i as [|i IH]; intros l le.
-      - lia.
-      - destruct l; auto.
-        cbn in le.
-        specialize (IH l ltac:(lia)).
-        cbn.
-        rewrite sumZ_seq_n.
-        rewrite Z_eta.
-        apply f_equal.
-        rewrite IH.
-        apply sumZ_exteq_proper; auto.
-        clear.
-        intros n.
-        replace (n + 1)%nat with (S n) by lia.
-        repeat
-          match goal with
-          | [|- context[Nat.ltb ?a ?b]] => destruct (Nat.ltb_spec a b)
-          | [|- context[Nat.leb ?a ?b]] => destruct (Nat.leb_spec a b)
-          | [|- context[Nat.eqb ?a ?b]] => destruct (Nat.eqb_spec a b)
-          end;
-          cbn in *; lia.
-    }.
-        destruct (n <? i)%nat eqn:lt; [apply Nat.ltb_lt in lt|apply Nat.ltb_ge in lt].
-        Search (S _ =? S _).
-        rewrite
-        cbn.
-        Search (_ + 1 <=? _).
-        cbn.
-        cbn.
-      cbn -[Nat.ltb Z.mul] in *.
-      rewrite sumZ_seq_n.
-      destruct (Nat.ltb_spec 0 i); try lia.
-      rewrite <- IH.
-      unfold id.
-      replace (length l + (i - length l))%nat with i in * by lia.
-      rewrite firstn_nil in H.
-      rewrite app_nil_r in *.
-      rewrite H; cbn -[skipn Nat.ltb].
-
-      rewrite firstn_le_length
-    induction i as [|x xs IH].
-    - rewrite firstn_nil. auto.
-    - cbn
-*)
-  Local Open Scope Z.
-
-  (*
-  Local Open Scope ffield.
-  Lemma mul_votes (sks : list Z) :
-    prod (map (fun '(sk, rk) => pow rk sk)
-                 (zip sks (reconstructed_keys (map compute_public_key sks))))
-    == 1.
-  Proof.
-
-
-  Lemma sum_pks (sks : list Z) :
-    sumZ (fun '(sk, rk) => sk * log rk)%Z
-         (zip sks (reconstructed_keys (map compute_public_key sks))) exp= 0%Z.
-  Proof.
-    induction sks as [|sk sks IH]; cbn in *.
-    1: reflexivity.
-    setoid_replace
-      (1 * (inv (compute_public_key sk *
-                 prod (map compute_public_key sks)) *
-            compute_public_key sk))
-      with (inv (prod (map compute_public_key sks)))
-      by (field; auto).
-
-
-    replace (1 * pk) with pk by field.
-    replace (inv (pk * prod pks) * pk) with (inv (prod pks)); cycle 1.
-    { field. intuition. }
-    replace (1 * (inv (prod pks))) with (inv (prod pks)); cycle 1.
-    { field. intuition. }
-
-    destruct units as [unit units].
-    rewrite <- log_mul; auto.
-    rewrite <- Z.add_mod_idemp_l by lia.
-    rewrite <- (log_mul pk); auto.
-    set (blah := match mod_inv _ _ * _ with _ => _ end).
-
-  Lemma rks_alt sks n :
-    All IsUnit sks ->
-    (n < length sks)%nat ->
-    reconstructed_key (map compute_public_key sks) n =
-    generator ^ (sumZ id (firstn n sks) - sumZ id (skipn (S n) sks)) mod modulus.
-  Proof.
-    intros.
-    induction n as [|n IH].
-    - destruct sks; cbn in *; try lia.
-      unfold reconstructed_key.
-      cbn.
-      rewrite eta_Z.
-
-      unfold id at 1.
-      replace (z + sumZ id sks - z) with (sumZ id sks) by lia.
-
-  Lemma sum_pks pks :
-    All IsUnit pks ->
-    sumZ (fun '(pk, rk) => log pk + log rk)
-         (zip pks (reconstructed_keys pks)) mod modulus = 0.
-  Proof.
-    intros units.
-    induction pks as [|pk pks IH]; auto.
-    cbn.
-    rewrite !eta_Z.
-    rewrite mod_inv_mod_idemp, mod_inv_mul.
-    destruct units as [unit units].
-    rewrite <- Z.add_mod_idemp_l by lia.
-    rewrite <- (log_mul pk); auto.
-    set (blah := match mod_inv _ _ * _ with _ => _ end).
-
-Fixpoint mod_prod (l : list Z) (m : Z) : Z :=
-  match l with
-  | [] => 1
-  | x :: xs => x * mod_prod xs m mod m
-  end.
-
-Fixpoint mod_pow_aux (a : bigZ) (x : positive) (m : bigZ) (r : bigZ) : bigZ :=
-  match x with
-  | x~0%positive => mod_pow_aux (BigZ.square a mod m) x m r
-  | x~1%positive => mod_pow_aux (BigZ.square a mod m) x m (r * a mod m)
-  | _ => r * a mod m
-  end.
-
-Hint Rewrite BigZ.square_spec BigZ.spec_pow_pos : zsimpl.
-Hint Rewrite BigN.spec_of_pos : nsimpl.
-
-Global Instance BigZ_square_wd :
-  Proper (BigZ.eq ==> BigZ.eq) BigZ.square.
-Proof.
-  intros a b eq.
-  autorewrite with zsimpl in *.
-  now rewrite eq.
-Qed.
-
-Global Instance mod_pow_aux_wd :
-  Proper (BigZ.eq ==> eq ==> BigZ.eq ==> BigZ.eq ==> BigZ.eq) mod_pow_aux.
-Proof.
-  (*intros a1 a2 elmeq ? x -> m1 m2 meq r1 r2 elmeq.*)
-  intros a1 a2 elmeq ? x ->.
-  revert a1 a2 elmeq.
-  induction x; intros a1 a2 elmeq m1 m2 meq r1 r2 elmeq.
-  - cbn.
-    apply IHx.
-    + rewrite elmeq, meq.
-      reflexivity.
-    + auto.
-    + rewrite elmeq, elmeq, meq.
-      reflexivity.
-  - cbn.
-    apply IHx.
-    + rewrite elmeq, meq.
-      reflexivity.
-    + auto.
-    + rewrite elmeq.
-      reflexivity.
-  - cbn.
-    rewrite elmeq, elmeq, meq.
-    reflexivity.
-Qed.
-
-Definition mod_pow (a x m : Z) : Z :=
-  match m with
-  | Z0 => 0
-  | _ =>
-    match x with
-    | Z0 => 1 mod m
-    | Zneg _ => 0
-    | Zpos x => [mod_pow_aux (BigZ.of_Z a) x (BigZ.of_Z m) 1]%bigZ
-    end
-  end.
-
-Local Open Scope Z.
-Lemma Z_pow_pos_mod_idemp a x m :
-  Z.pow_pos (a mod m) x mod m = Z.pow_pos a x mod m.
-Proof.
-  destruct (m =? 0) eqn:mzero.
-  {
-    apply Z.eqb_eq in mzero.
-    rewrite mzero.
-    now rewrite 2!Zmod_0_r.
-  }
-
-  apply Z.eqb_neq in mzero.
-
-  unfold Z.pow_pos.
-  assert (H: forall start l x, Pos.iter (Z.mul l) start x = start * Pos.iter (Z.mul l) 1 x).
-  {
-    clear.
-    intros start l x.
-    revert start.
-    induction x; intros start.
-    - cbn.
-      rewrite 2!IHx.
-      rewrite (IHx (Pos.iter (Z.mul l) 1 x)).
-      lia.
-    - cbn.
-      rewrite 2!IHx.
-      rewrite (IHx (Pos.iter (Z.mul l) 1 x)).
-      lia.
-    - cbn.
-      lia.
-  }
-
-  induction x.
-  - cbn.
-    rewrite (H _ (a mod m)).
-    rewrite (H _ a).
-    rewrite Z.mul_assoc.
-    assert (H2: forall a b c,
-               ((a mod m) * b * c) mod m = ((a mod m) * (b mod m) * (c mod m)) mod m).
-    {
-      clear.
-      intros.
-      rewrite <- Z.mul_assoc.
-      rewrite Zmult_mod_idemp_l.
-
-      rewrite <- Z.mul_assoc.
-      rewrite Zmult_mod_idemp_l.
-
-      rewrite 2!Z.mul_assoc.
-      rewrite (Z.mul_comm _ (c mod m)).
-      rewrite Zmult_mod_idemp_l.
-      rewrite Z.mul_assoc.
-      rewrite (Z.mul_comm _ (b mod m)).
-      rewrite Zmult_mod_idemp_l.
-      replace (b * (c * a)) with (a * b * c) by lia; auto.
-    }
-
-    rewrite H2.
-    rewrite IHx.
-    rewrite <- H2.
-
-    rewrite <- Z.mul_assoc.
-    now rewrite Zmult_mod_idemp_l.
-  - cbn.
-    rewrite H.
-    rewrite Z.mul_mod by auto.
-    rewrite IHx.
-    rewrite <- Z.mul_mod by auto.
-    now rewrite <- H.
-  - cbn.
-    rewrite 2!Z.mul_1_r.
-    now apply Z.mod_mod.
-Qed.
-
-Lemma Z_pow_mod_idemp a x m :
-  (a mod m)^x mod m = a^x mod m.
-Proof.
-  destruct x; auto.
-  cbn.
-  apply Z_pow_pos_mod_idemp.
-Qed.
-
-Lemma mod_pow_aux_spec a x m r :
-  m != 0 ->
-  mod_pow_aux a x m r == r * BigZ.pow_pos a x mod m.
-Proof.
-  cbn.
-  intros nonzero.
-  revert a r.
-  induction x; intros a r.
-  - cbn.
-    specialize (IHx ((a * a) mod m) ((r * a) mod m))%bigZ.
-    autorewrite with zsimpl.
-    rewrite IHx.
-    unfold "==".
-    autorewrite with zsimpl.
-    cbn -[Z.pow_pos].
-    rewrite <- Z.mul_mod_idemp_r by auto.
-    rewrite Z_pow_pos_mod_idemp.
-    rewrite <- Z.mul_mod by auto.
-    replace (x~1)%positive with (x*2+1)%positive by lia.
-    rewrite Zpower_pos_is_exp.
-    cbn.
-    rewrite 2!Z.pow_pos_fold.
-    rewrite Z.pow_mul_l.
-    rewrite <- Z.pow_add_r by (auto with zarith).
-    rewrite Zred_factor1.
-    f_equal.
-    lia.
-  - cbn.
-    rewrite IHx.
-    unfold "==".
-    autorewrite with zsimpl.
-    cbn -[Z.pow_pos].
-    rewrite <- Zmult_mod_idemp_r.
-    rewrite Z_pow_pos_mod_idemp.
-    rewrite Zmult_mod_idemp_r.
-    replace (x~0)%positive with (x*2)%positive by lia.
-    rewrite 2!Z.pow_pos_fold.
-    rewrite Z.pow_mul_l.
-    rewrite <- Z.pow_add_r by (auto with zarith).
-    now rewrite Zred_factor1.
-  - cbn.
-    unfold "==".
-    autorewrite with zsimpl.
-    f_equal; lia.
-Qed.
-
-Lemma mod_pow_spec a x m :
-  mod_pow a x m = a^x mod m.
-Proof.
-  unfold mod_pow.
-  destruct m.
-  - now rewrite Zmod_0_r.
-  - destruct x; auto.
-    rewrite mod_pow_aux_spec.
-    + autorewrite with zsimpl.
-      f_equal.
-      cbn.
-      destruct (Z.pow_pos _ _); auto.
-    + intro cont.
-      unfold "==" in *.
-      cbn in *.
-      autorewrite with nsimpl in cont.
-      lia.
-  - destruct x; auto.
-    rewrite mod_pow_aux_spec.
-    + autorewrite with zsimpl.
-      f_equal.
-      cbn.
-      destruct (Z.pow_pos _ _); auto.
-    + intro cont.
-      unfold "==" in *.
-      cbn in *.
-      autorewrite with nsimpl in cont.
-      lia.
-Qed.
-
-(* Find y such that x*y = 1 mod m *)
-Definition mod_inv (x m : Z) : Z :=
-  mod_pow x (m - 2) m.
-
-Compute (mod_inv (mod_pow 33 47 59) 59).
-Compute (FGroup.i (ZPGroup 59 ltac:(lia)) (gpow 33 (ZPGroup 59 ltac:(lia)) 47)).
-Compute (inv 33 (ZPGroup 47 ltac:(lia)) (-1)).
-
-Lemma mod_inv_spec x m :
-  prime m ->
-  x mod m <> 0 ->
-  (x * mod_inv x m) mod m = 1.
-Proof.
-  intros is_prime xnm.
-  pose proof (prime_ge_2 _ is_prime).
-  unfold mod_inv.
-  rewrite (mod_pow_spec x (m - 2) m).
-  rewrite Z.mul_mod_idemp_r by lia.
-  rewrite <- Z.pow_succ_r by lia.
-  replace (Z.succ (m - 2)) with (m - 1) by lia.
-  (* Use proof of Euler's theorem from Coqprime *)
-  rewrite <- (Euler.prime_phi_n_minus_1 _ is_prime).
-  apply phi_power_is_1; try lia.
-  apply rel_prime_sym.
-  apply prime_rel_prime; auto.
-  intros div.
-  pose proof (Zdivide_mod _ _ div).
-  tauto.
-Qed.
-
-Lemma mod_inv_mod_idemp (x m : Z) :
-  mod_inv (x mod m) m = mod_inv x m.
-Proof.
-  unfold mod_inv.
-  rewrite 2!mod_pow_spec.
-  now rewrite Z_pow_mod_idemp.
-Qed.
-
-Lemma mod_inv_mul a b m :
-  mod_inv (a * b) m =
-  (mod_inv a m * mod_inv b m) mod m.
-Proof.
-  unfold mod_inv.
-  now rewrite !mod_pow_spec, Z.pow_mul_l, Zmult_mod.
-Qed.
-
-Section Modulus.
-  Context (modulus : Z).
-  Context (is_prime : prime modulus).
-
-  Let m_ge_2 := prime_ge_2 _ is_prime.
-
-  Definition IsUnit (z : Z) : Prop :=
-    z mod modulus <> 0.
-
-  Record IsGenerator g : Prop :=
-    build_is_generator {
-      generator_between : 0 < g < modulus;
-      generator_generates x :
-        IsUnit x -> exists! e, 0 <= e < modulus /\ g ^ e mod modulus = x mod modulus;
-      generator_order : g ^ (modulus - 1) mod modulus = 1;
-    }.
-
-  Context (generator : Z).
-  Context (is_generator : IsGenerator generator).
-
-  Definition Z_encode (z : Z) : nat :=
-    Z.to_nat (if z <? 0 then -z * 2 + 1 else z * 2).
-  Definition Z_decode (n : nat) : Z :=
-    if Nat.even n then
-      Z.of_nat n / 2
-    else
-      -Z.of_nat n / 2 + 1.
-  Lemma Z_decode_encode (z : Z) : Z_decode (Z_encode z) = z.
-  Proof.
-    unfold Z_encode, Z_decode.
-    destruct (z <? 0) eqn:lt0;
-      [apply Z.ltb_lt in lt0|apply Z.ltb_ge in lt0].
-    - rewrite Z2Nat.id by lia.
-      rewrite Z2Nat.inj_add; try lia.
-      rewrite Z2Nat.inj_mul; try lia.
-      cbn; unfold Pos.to_nat; cbn.
-      rewrite Nat.add_comm, Nat.mul_comm at 1.
-      rewrite Nat.even_mul_add_2.
-      cbn.
-      rewrite Z.opp_add_distr, Z.mul_opp_l, Z.opp_involutive.
-      cbn.
-      rewrite Z.div_add_l by lia.
-      cbn.
-      lia.
-    - rewrite Z2Nat.inj_mul by lia.
-      cbn; unfold Pos.to_nat; cbn.
-      rewrite Nat.even_mul; cbn; rewrite Bool.orb_true_r.
-      rewrite Nat2Z.inj_mul.
-      cbn; unfold Pos.to_nat; cbn.
-      rewrite Z.div_mul by lia.
-      rewrite Z2Nat.id; auto.
-  Qed.
-
-  Lemma deunique {A} (P : A -> Prop) :
-    (exists! x, P x) -> exists x, P x.
-  Proof.
-    intros [x []].
-    exists x; auto.
-  Qed.
-
-  Definition log_with_spec (x : Z) :
-    IsUnit x ->
-    { e : Z | 0 <= e < modulus /\ generator ^ e mod modulus = x mod modulus }.
-  Proof.
-    intros isunit.
-    refine (constructive_definite_ground_description
-              Z Z_encode Z_decode Z_decode_encode
-              _ _ (generator_generates _ is_generator _ isunit)).
-    intros e.
-    destruct ((e >=? 0) && (e <? modulus) && (generator ^ e mod modulus =? x mod modulus))%bool eqn:test.
-    - left.
-      apply Bool.andb_true_iff in test; destruct test as [test test3].
-      apply Bool.andb_true_iff in test; destruct test as [test1 test2].
-      apply Z.geb_le in test1.
-      apply Z.ltb_lt in test2.
-      apply Z.eqb_eq in test3.
-      tauto.
-    - right.
-      apply Bool.andb_false_iff in test; destruct test as [test|test].
-      + apply Bool.andb_false_iff in test; destruct test as [test|test].
-        * rewrite Z.geb_leb in test.
-          apply Z.leb_gt in test.
-          lia.
-        * apply Z.ltb_ge in test.
-          lia.
-      + apply Z.eqb_neq in test.
-        tauto.
-  Defined.
-
-  Definition log (x : Z) : Z.
-  Proof.
-    destruct (Z.eq_dec (x mod modulus) 0) as [eq|ne].
-    - exact 0.
-    - exact (proj1_sig (log_with_spec x ne)).
-  Defined.
-
-  Lemma log_spec x :
-    IsUnit x ->
-    0 <= log x < modulus /\
-    generator ^ log x mod modulus = x mod modulus.
-  Proof.
-    intros is_unit.
-    unfold log.
-    destruct (Z.eq_dec _ _).
-    - contradiction.
-    - apply (proj2_sig (log_with_spec x n)).
-  Qed.
-
-  Lemma log_mul x y :
-    IsUnit x ->
-    IsUnit y ->
-    log (x * y) = (log x + log y) mod modulus.
-  Proof.
-    Admitted.
-
-  Lemma log_mod x :
-    log x mod modulus = log x.
-  Proof.
-    unfold log.
-    destruct (Z.eq_dec (x mod modulus) 0) as [eq|ne]; auto.
-    pose proof (proj2_sig (log_with_spec x ne)) as H.
-    cbn in H.
-    destruct H as [H _].
-    rewrite Z.mod_small; auto.
-  Qed.
-
-  Definition compute_public_key (sk : Z) : Z :=
-    mod_pow generator sk modulus.
-
-  Definition reconstructed_key (pks : list Z) (n : nat) : Z :=
-    let lprod := mod_prod (firstn n pks) modulus in
-    let rprod := mod_inv (mod_prod (skipn (S n) pks) modulus) modulus in
-    (lprod * rprod) mod modulus.
-
-  Fixpoint reconstructed_keys_aux
-           (pks : list Z) (lprod rprod : Z) : list Z :=
-    match pks with
-    | [] => []
-    | pk :: tl =>
-      let rprod := rprod * pk in
-      let rk := lprod * rprod mod modulus in
-      rk :: reconstructed_keys_aux tl (lprod * pk) rprod
-    end.
-
-  Definition reconstructed_keys (pks : list Z) : list Z :=
-    let rprod := mod_inv (mod_prod pks modulus) modulus in
-    reconstructed_keys_aux pks 1 rprod.
-
-  Lemma reconstructed_keys_aux_nth pks1 pk pks2 :
-    IsUnit pk ->
-    reconstructed_key (pks1 ++ pk :: pks2) (length pks1) =
-    hd 0 (reconstructed_keys_aux (pk :: pks2)
-                                 (mod_prod pks1 modulus)
-                                 (mod_inv (mod_prod (pk :: pks2) modulus) modulus)).
-  Proof.
-    intros unit.
-    unfold reconstructed_key.
-    replace (length pks1) with (length pks1 + 0)%nat at 1 by lia.
-    rewrite firstn_app_2; cbn.
-    rewrite app_nil_r.
-    replace (match pks1 ++ pk :: pks2 with | [] => [] | _ :: l => skipn (length pks1) l end)
-      with pks2; cycle 1.
-    { clear; induction pks1; auto. }
-    rewrite mod_inv_mod_idemp, mod_inv_mul.
-    rewrite <- (Z.mul_mod_idemp_r _ ((mod_inv pk modulus * mod_inv _ _) mod _ * pk)) by lia.
-    rewrite Z.mul_mod_idemp_l by lia.
-    replace (mod_inv pk _ * mod_inv _ _ * pk)
-      with (pk * mod_inv pk modulus * mod_inv (mod_prod pks2 modulus) modulus)
-      by lia.
-    rewrite <- (Z.mul_mod_idemp_l (pk * _)) by lia.
-    rewrite mod_inv_spec by auto.
-    rewrite Z.mul_1_l.
-    now rewrite Z.mul_mod_idemp_r by lia.
-  Qed.
-
-  Lemma eta_Z (z : Z) :
-    match z with
-    | Z0 => Z0
-    | Zpos p => Zpos p
-    | Zneg p => Zneg p
-    end = z.
-  Proof. now destruct z. Qed.
-
-  Lemma rks_alt sks n :
-    All IsUnit sks ->
-    (n < length sks)%nat ->
-    reconstructed_key (map compute_public_key sks) n =
-    generator ^ (sumZ id (firstn n sks) - sumZ id (skipn (S n) sks)) mod modulus.
-  Proof.
-    intros.
-    induction n as [|n IH].
-    - destruct sks; cbn in *; try lia.
-      unfold reconstructed_key.
-      cbn.
-      rewrite eta_Z.
-
-      unfold id at 1.
-      replace (z + sumZ id sks - z) with (sumZ id sks) by lia.
-
-
-  Lemma sum_pks pks :
-    All IsUnit pks ->
-    sumZ (fun '(pk, rk) => log pk + log rk)
-         (zip pks (reconstructed_keys pks)) mod modulus = 0.
-  Proof.
-    intros units.
-    induction pks as [|pk pks IH]; auto.
-    cbn.
-    rewrite !eta_Z.
-    rewrite mod_inv_mod_idemp, mod_inv_mul.
-    destruct units as [unit units].
-    rewrite <- Z.add_mod_idemp_l by lia.
-    rewrite <- (log_mul pk); auto.
-    set (blah := match mod_inv _ _ * _ with _ => _ end).
-
-
-  (*
-  Lemma reconstructed_keys_nth pks n :
-    All IsUnit pks ->
-    nth n (reconstructed_keys pks) 0 = reconstructed_key pks n.
-  Proof.
-    intros units.
-    assert (exists pref pk suf,
-               pref ++ pk :: suf = pks /\
-               length pref = n /\
-               IsUnit pk).
-    { admit. }
-    destruct H as [pref [pk [suf [<- [<- ?]]]]].
-    rewrite reconstructed_keys_aux_nth by auto.
-    unfold reconstructed_keys.
-    cbn.
-    fold (mod_prod suf modulus).
-    fold (reconstructed_keys_aux pref
-    fold (reconstructed_keys
-    unfold hd.
-    cbn.
-    induction n as [|n IH].
-    - cbn.
-    unfold reconstructed_keys.
-*)
-
-  Lemma map_reconstructed_key pks :
-    map (fun i => reconstructed_key
-    map reconstructed_key
-
-  Lemma prime_pow a b : b >= 0 -> (modulus | a ^ b) -> (modulus | a).
-  Proof.
-    intros nonnegative divides.
-    destruct b as [|e|e].
-    - pose proof (prime_ge_2 _ is_prime).
-      apply Z.divide_1_r in divides.
-      destruct divides; lia.
-    - induction e as [|e IH] using Pos.peano_ind.
-      + now rewrite Z.pow_1_r in divides.
-      + rewrite Pos2Z.inj_succ in divides.
-        rewrite <- Z.add_1_l in divides.
-        rewrite Z.pow_add_r in divides; [|lia|lia].
-        rewrite Z.pow_1_r in divides.
-        destruct (prime_mult _ is_prime _ _ divides); auto.
-    - lia.
-  Qed.
-
-  Lemma pow_0 b x :
-    x >= 0 ->
-    b ^ x mod modulus = 0 ->
-    b mod modulus = 0.
-  Proof.
-    intros nonneg eq.
-    pose proof (prime_ge_2 _ is_prime).
-    apply Z.mod_divide; [lia|].
-    apply Z.mod_divide in eq; [|lia].
-    apply prime_pow with x; auto.
-  Qed.
-  (*
-Lemma generator_pos b x :
-  0 <= x ->
-  b mod p <> 0 ->
-  b ^ x mod p <> 0.
-Proof.
-  intros x_nonneg b_noncongruent.
-  pose proof (prime_ge_2 _ is_prime).
-  (*destruct is_generator as [g_between g_order].*)
-  assert (b ^ x mod p <> 0).
-  {
-    apply pow_0 in eq; [|lia].
-    apply Z.mod_divide in eq; [|lia].
-    destruct eq as [k eq].
-    subst.
-    destruct k; cbn in *.
-    - cbn in *; lia.
-    - rewrite Z.mul_comm in g_between.
-      pose proof (proj1 (Z.le_mul_diag_r modulus (Z.pos p) ltac:(lia)) ltac:(lia)).
-      lia.
-    - assert (Z.neg p <= -1) by lia.
-      pose proof (proj1 (Z.le_mul_diag_l (Z.neg p) modulus ltac:(lia)) ltac:(lia)).
-      lia.
-  }
-
-  pose proof (Z.mod_pos_bound (generator ^ n) modulus ltac:(lia)).
-  lia.
-Qed.
-   *)
-
-  Lemma log z :
-    z <> 0 ->
-    exists! e, generator ^ e mod modulus = z mod modulus.
-  Proof.
-    Admitted.
-
-  Definition compute_public_vote (rk sk : Z) (sv : bool) : Z :=
-    (mod_pow rk sk modulus * if sv then generator else 1) mod modulus.
-
-  Lemma generator_pos x :
-    0 <= x ->
-    generator ^ x mod modulus > 0.
-  Proof.
-    intros nonneg.
-    destruct is_generator as [between _].
-    assert (generator^x mod modulus <> 0).
-    {
-      intros eq.
-      apply pow_0 in eq; [|lia].
-      apply Z.mod_divide in eq; [|lia].
-      destruct eq as [k eq].
-      subst.
-      destruct k as [|k|k]; cbn -[Z.mul] in *.
-      - cbn in *; lia.
-      - rewrite Z.mul_comm in between.
-        pose proof (proj1 (Z.le_mul_diag_r modulus (Z.pos k) ltac:(lia)) ltac:(lia)).
-        lia.
-      - assert (Z.neg k <= -1) by lia.
-        pose proof (proj1 (Z.le_mul_diag_l (Z.neg k) modulus ltac:(lia)) ltac:(lia)).
-        lia.
-    }
-
-    pose proof (Z.mod_pos_bound (generator^x) modulus ltac:(lia)).
-    lia.
-  Qed.
-
-  Lemma AllUnits_pks sks :
-    AllUnits sks -> AllUnits (map compute_public_key sks).
-  Proof.
-    intros sks_pos.
-    apply AllUnits_map; auto.
-    intros x x_gt.
-    unfold compute_public_key.
-    rewrite mod_pow_spec.
-    apply generator_pos; lia.
-  Qed.
-
-  (*
-  Lemma rks_prod (sks : list Z) (pks : list Z) :
-    AllUnits sks ->
-    pks = map compute_public_key sks ->
-    prodZ (fun i => (reconstructed_key pks i) ^ nth i sks 0) (seq 0 (length sks)) mod modulus = 1.
-  Proof.
-    intros sks_pos pks_eq.
-    assert (pks_pos: AllUnits pks) by (subst; auto using AllUnits_pks).
-
-    assert (exists exps, map (fun exp => generator ^ exp mod modulus) exps =
-                         map (fun i => reconstructed_key pks i) (seq 0 (length pks))).
-    { clear -is_prime is_generator pks_pos.
-      induction pks as [|pk pks IH].
-      - now exists [].
-      - apply AllUnits_cons_r in pks_pos.
-        destruct pks_pos as [pk_pos pks_pos].
-        destruct IH as [tl IH]; [tauto|].
-        destruct (log pk ltac:(lia)) as [e [e_eq e_uniq]].
-        exists (e :: tl).
-        cbn.
-        rewrite IH.
-
-                                 k=
-                               reconstructed_key pks
-                                                 pose proof (prime_ge_2 _ modulus_prime).
-                               generalize 0%nat.
-                               induction sks as [|sk sks IH]; intros n.
-                               - apply Z.mod_1_l; lia.
-                               - apply AllUnitsKeys_cons in nonzero.
-                                 destruct nonzero as [sk_nonzero nonzero].
-                                 specialize (IH nonzero).
-                                 cbn.
-
-*)
-*)
-*)
-End WithFField.
-
-Section Zp.
+Module Zp.
   Local Open Scope Z.
 
   Fixpoint mod_pow_pos_aux (a : Z) (x : positive) (m : Z) (r : Z) : Z :=
@@ -1864,6 +943,19 @@ Section Zp.
     tauto.
   Qed.
 
+  Lemma mod_pow_fermat a p :
+    prime p ->
+    a mod p <> 0 ->
+    mod_pow a (p - 1) p = 1.
+  Proof.
+    intros isprime ap.
+    pose proof (prime_ge_2 _ isprime).
+    pose proof (mod_pow_pos_fermat _ _ isprime ap).
+    destruct p; try lia.
+    destruct (Z.pos p - 1) eqn:?; try lia.
+    assumption.
+  Qed.
+
   Lemma mod_pow_pos_exp_plus a x x' p :
     mod_pow_pos a (x + x') p = mod_pow_pos a x p * mod_pow_pos a x' p mod p.
   Proof.
@@ -1875,7 +967,6 @@ Section Zp.
       rewrite Z.pow_add_r by lia.
       now rewrite Z.mul_mod by auto.
   Qed.
-
   Lemma mod_pow_pos_exp_mul a x x' p :
     mod_pow_pos a (x * x') p = mod_pow_pos (mod_pow_pos a x p) x' p.
   Proof.
@@ -1888,24 +979,53 @@ Section Zp.
       now rewrite <- Z.pow_mul_r by lia.
   Qed.
 
-  Lemma mod_pow_pos_1_l x p :
-    mod_pow_pos 1 x p = 1 mod p.
+  Lemma mod_pow_pos_aux_1_l x p r :
+    mod_pow_pos_aux 1 x p r = r mod p.
   Proof.
     destruct (Z.eq_dec p 0) as [->|?].
-    - unfold mod_pow_pos.
-      cbn.
-      generalize 1 at 1.
-      generalize 1 at 1.
-      induction x; intros a r; auto.
-      + cbn.
-        now rewrite IHx.
-      + cbn.
-        now rewrite IHx.
-      + cbn.
-        now rewrite Zmod_0_r.
-    - rewrite mod_pow_pos_spec by auto.
-      rewrite Z.pow_pos_fold.
-      now rewrite Z.pow_1_l by lia.
+    - now rewrite mod_pow_pos_aux_0_r, Zmod_0_r.
+    - revert r.
+      induction x; intros r; cbn.
+      + rewrite mod_pow_pos_aux_mod_idemp.
+        rewrite Z.mul_1_r.
+        rewrite IHx.
+        apply Z.mod_mod; auto.
+      + rewrite mod_pow_pos_aux_mod_idemp.
+        apply IHx.
+      + now rewrite Z.mul_1_r.
+  Qed.
+  Lemma mod_pow_pos_1_l x p :
+    mod_pow_pos 1 x p = 1 mod p.
+  Proof. apply mod_pow_pos_aux_1_l. Qed.
+  Lemma mod_inv_1_l p :
+    mod_inv 1 p = 1 mod p.
+  Proof. apply mod_pow_pos_1_l. Qed.
+  Lemma mod_pow_1_l x p :
+    mod_pow 1 x p = 1 mod p.
+  Proof.
+    destruct x; auto; cbn.
+    - apply mod_pow_pos_1_l.
+    - rewrite mod_pow_pos_1_l, mod_inv_mod_idemp.
+      apply mod_inv_1_l.
+  Qed.
+
+  Lemma mod_pow_pos_aux_1_r a p r :
+    mod_pow_pos_aux a 1 p r = a * r mod p.
+  Proof.
+    cbn.
+    now rewrite Z.mul_comm.
+  Qed.
+  Lemma mod_pow_pos_1_r a p :
+    mod_pow_pos a 1 p = a mod p.
+  Proof.
+    cbn -[Z.mul].
+    now rewrite Z.mul_1_l.
+  Qed.
+  Lemma mod_pow_1_r a p :
+    mod_pow a 1 p = a mod p.
+  Proof.
+    cbn -[Z.mul].
+    now rewrite Z.mul_1_l.
   Qed.
 
   Lemma mod_pow_pos_succ_r a x p :
@@ -2017,51 +1137,21 @@ Section Zp.
       rewrite mod_pow_pos_mod; auto.
   Qed.
   Hint Resolve mod_pow_nonzero : core.
+  Lemma mod_pow_pos_mod_nonzero a x p :
+    mod_pow_pos a x p <> 0 ->
+    mod_pow_pos a x p mod p <> 0.
+  Proof. rewrite mod_pow_pos_mod; auto. Qed.
+  Lemma mod_inv_mod_nonzero a p :
+    mod_inv a p <> 0 ->
+    mod_inv a p mod p <> 0.
+  Proof. rewrite mod_inv_mod; auto. Qed.
+  Lemma mod_pow_mod_nonzero a x p :
+    mod_pow a x p <> 0 ->
+    mod_pow a x p mod p <> 0.
+  Proof. rewrite mod_pow_mod; auto. Qed.
+  Hint Resolve mod_pow_pos_mod_nonzero mod_inv_mod_nonzero mod_pow_mod_nonzero : core.
 
-  Section MyInd.
-    Context (P : Z -> Prop).
-    Context (case0 : P 0).
-    Context (case01 : P 0 -> P (Z.pos 1)).
-    Context (caseS : forall p, P (Z.pos p) -> P (Z.pos p + 1)).
-    Context (case_neg : forall p, P (Z.pos p) -> P (Z.neg p)).
-
-    Definition measure (z : Z) : nat :=
-      if z <? 0 then Z.to_nat (-z + 1) else Z.to_nat z.
-
-    Lemma measure0 z : measure z = 0%nat -> z = 0.
-    Proof.
-      intros mz.
-      destruct z; cbn in *; lia.
-    Qed.
-
-    Lemma my_ind (z : Z) : P z.
-    Proof.
-      enough (forall x, measure x <= measure z -> P x)%nat.
-      { apply H; lia. }
-
-      induction (measure z).
-      - intros x mx.
-        rewrite (measure0 x ltac:(lia)).
-        apply case0.
-      - intros x mx.
-        destruct x.
-        + apply case0.
-        + destruct (Pos.eq_dec p 1) as [->|?].
-          * apply (case01 case0).
-          * specialize (caseS (p - 1)).
-            replace (Z.pos (p - 1) + 1) with (Z.pos p) in caseS by lia.
-            apply caseS.
-            apply IHn.
-            cbn in *.
-            lia.
-        + apply case_neg.
-          apply IHn.
-          cbn in *.
-          lia.
-    Qed.
-  End MyInd.
-
-  Lemma Zp_mul_both_l a b c p :
+  Lemma mod_mul_both_l a b c p :
     prime p ->
     c mod p <> 0 ->
     c * a mod p = c * b mod p ->
@@ -2080,10 +1170,26 @@ Section Zp.
     now rewrite eq.
   Qed.
 
-  Lemma mod_pow_succ_r a x p :
+  Lemma mod_inv_mul a b p :
     prime p ->
     a mod p <> 0 ->
-    mod_pow a (1 + x) p = a * mod_pow a x p mod p.
+    b mod p <> 0 ->
+    mod_inv (a * b) p = mod_inv b p * mod_inv a p mod p.
+  Proof.
+    intros isprime ap0 bp0.
+    pose proof (prime_ge_2 _ isprime).
+    unfold mod_inv.
+    rewrite !mod_pow_pos_spec, !Z.pow_pos_fold.
+    rewrite Z.pow_mul_l.
+    rewrite Z.mul_mod by lia.
+    rewrite <- !Z.pow_pos_fold, <- !mod_pow_pos_spec.
+    now rewrite Z.mul_comm.
+  Qed.
+
+  Lemma mod_pow_succ a x p :
+    prime p ->
+    a mod p <> 0 ->
+    mod_pow a (Z.succ x) p = a * mod_pow a x p mod p.
   Proof.
     intros isprime ap0.
     pose proof (prime_ge_2 _ isprime).
@@ -2094,7 +1200,7 @@ Section Zp.
       destruct a; auto.
     - cbn -[Pos.add].
       rewrite mod_pow_pos_succ_r.
-      now replace (1 + p0)%positive with (Pos.succ p0) by lia.
+      now replace (p0 + 1)%positive with (Pos.succ p0) by lia.
     - cbn.
       destruct (Pos.eq_dec p0 1) as [->|?].
       + cbn -[Z.mul].
@@ -2105,16 +1211,35 @@ Section Zp.
       + rewrite Z.pos_sub_lt by lia.
         cbn.
         rewrite <- mod_inv_mod.
-        apply Zp_mul_both_l with (mod_inv a p); auto.
-        * rewrite mod_inv_mod; auto.
-        * rewrite Z.mul_assoc.
-          rewrite <- (Z.mul_mod_idemp_l (mod_inv a p * a)) by lia.
-          rewrite (Z.mul_comm _ a).
-          rewrite mul_mod_inv by auto.
+        apply mod_mul_both_l with (mod_inv a p); auto.
+        rewrite Z.mul_assoc.
+        rewrite <- (Z.mul_mod_idemp_l (mod_inv a p * a)) by lia.
+        rewrite (Z.mul_comm _ a).
+        rewrite mul_mod_inv by auto.
+        rewrite <- mod_inv_mul by auto.
+        rewrite Z.mul_comm.
+        rewrite <- mod_inv_mod_idemp.
+        rewrite mod_pow_pos_succ_r.
+        replace (Pos.succ (p0 - 1)) with p0 by lia.
+        now rewrite Z.mul_1_l, mod_inv_mod.
+  Qed.
 
-        destruct (Z.pos_sub 1 p0) eqn:?; try lia.
-      destruct p0.
-      unfold mod_pow.
+  Lemma mod_pow_pred a x p :
+    prime p ->
+    a mod p <> 0 ->
+    mod_pow a (Z.pred x) p = mod_inv a p * mod_pow a x p mod p.
+  Proof.
+    intros isprime ap0.
+    pose proof (prime_ge_2 _ isprime).
+    rewrite <- mod_pow_mod.
+    apply mod_mul_both_l with a; auto.
+    rewrite <- mod_pow_succ by auto.
+    replace (Z.succ (Z.pred x)) with x by lia.
+    rewrite Z.mul_assoc.
+    rewrite <- Z.mul_mod_idemp_l by lia.
+    rewrite mul_mod_inv by auto.
+    now rewrite Z.mul_1_l, mod_pow_mod.
+  Qed.
 
   Lemma mod_pow_exp_plus a x x' p :
     prime p ->
@@ -2124,220 +1249,202 @@ Section Zp.
     intros isprime ap0.
     pose proof (prime_ge_2 _ isprime).
     revert x'.
-    induction x using my_ind; intros x'.
+    induction x using Z.peano_ind; intros x'.
     - cbn.
       rewrite Z.mod_1_l by lia.
       rewrite Z.mul_1_l.
       now rewrite mod_pow_mod by lia.
-    - cbn.
-    - rewrite <- Z.add_assoc.
+    - replace (Z.succ x + x') with (Z.succ (x + x')) by lia.
+      rewrite mod_pow_succ by auto.
       rewrite IHx.
-      unfold mod_pow.
-      repeat rewrite mod_pow_spec by auto.
-      rewrite mod_pow_spec.
-      rewrite Z.mul_comm.
-      rewrite Z.add_comm.
-      replace (x + 1) with (1 + x) by lia.
-      unfold mod_pow.
-   unfold mod_pow, mod_inv.
-    destruct x, x'; cbn.
-    all: try rewrite !Z.mod_1_l by lia; auto.
-    all: try rewrite !Z.mul_1_l; try rewrite !Z.mul_1_r.
-    all: try rewrite !mod_pow_pos_mod; auto.
-    - apply mod_pow_pos_exp_plus.
-    - rewrite Z.pos_sub_spec.
-      destruct (Pos.compare_spec p0 p1) as [<-|?|?].
-      + fold (mod_inv (mod_pow_pos a p0 p) p).
-        rewrite mul_mod_inv; auto.
-        rewrite mod_pow_pos_mod.
-        now apply mod_pow_pos_nonzero.
-      + fold (mod_inv (mod_pow_pos a (p1 - p0) p) p).
-        fold (mod_inv (mod_pow_pos a p1 p) p).
-        rewrite <- !(mod_pow_pos_exp_mul a).
-        rewrite <- mod_pow_pos_exp_plus.
-        rewrite Pos.mul_sub_distr_r by lia.
-        rewrite Pos.add_comm.
-        rewrite mod_pow_pos_exp_plus.
+      rewrite Z.mul_mod_idemp_r by lia.
+      rewrite Z.mul_assoc.
+      rewrite <- Z.mul_mod_idemp_l by lia.
+      now rewrite <- mod_pow_succ by auto.
+    - replace (Z.pred x + x') with (x + Z.pred x') by lia.
+      rewrite IHx.
+      rewrite !mod_pow_pred by auto.
+      rewrite Z.mul_mod_idemp_l, Z.mul_mod_idemp_r by lia.
+      apply f_equal2; lia.
+  Qed.
 
-        rewrite mod_pow_pos_exp_sub.
-        rewrite Pos2Z.inj_sub by auto.
-        destruct (Z.eq_dec a 0) as [->|?]; [rewrite Z.mod_0_l in ap0; auto; congruence|].
-        rewrite Z.pow_sub_r by lia.
-        apply Pos.compare_lt in cmp.
-        destruct (Z.pos_sub p0 o1)
-        rewrite mod_pow_pos_spec, Z.pow_pos_fold.
-        rewrite Z.pos_sub_diag; cbn.
-        rewrite mod_pow_pos_succ_r.
-        rewrite <- mod_pow_pos_exp_mul.
-        destruct (Z.eq_dec p 2) as [->|?].
-        * cbn.
-          destruct
-
-        replace (Pos.succ (Z.to_pos (p - 2))) with (Z.to_pos (p - 1)) by lia.
-        rewrite <- mod_pow_pos_exp_mul.
-        rewrite mod_pow_
-
-    all: cbn.
-    destruct x
-    destruct p; auto.
-    all: destruct (x + x') eqn:?, x, x'.
-    all: try rewrite Z.pow_0_r, !Z.mod_1_l by lia; auto; try lia.
-    - replace p1 with p0 by lia.
-
-    destruct (Z.eq_dec p 0) as [->|?]; auto.
-
-  (*
-  Lemma mod_pow_pos_exp a x p k :
+  Lemma mod_inv_involutive a p :
     prime p ->
     a mod p <> 0 ->
-    mod_pow_pos a x p = mod_pow_pos a (x + Z.to_pos (k *  Z.p (Z.to_pos (Z.pos x mod (p - 1))) p.
+    mod_inv (mod_inv a p) p = a mod p.
   Proof.
-    intros isprime ap0 xp0.
-    pose proof (prime_ge_2 _ isprime).
-    destruct (Z.pos x <? (p - 1)) eqn:lt.
-    {
-      apply Z.ltb_lt in lt.
-      now rewrite Z.mod_small by lia.
-    }
-
-    apply Z.ltb_ge in lt.
-    change x with (Z.to_pos (Z.pos x)) at 1.
-    rewrite (Z.quot_rem' (Z.pos x) (p - 1)) at 1.
-    rewrite Z2Pos.inj_add; cycle 1.
-    + apply Z.mul_pos_pos; try lia.
-      apply Z.quot_str_pos; lia.
-    + rewrite Z.rem_mod_nonneg by lia.
-      pose proof (Z.mod_pos_bound (Z.pos x) (p - 1) ltac:(lia)).
-      lia.
-    + rewrite Z2Pos.inj_mul; cycle 1.
-      * lia.
-      * apply Z.quot_str_pos; lia.
-      * rewrite mod_pow_pos_exp_plus by lia.
-        rewrite mod_pow_pos_exp_mul by lia.
-        rewrite mod_pow_pos_fermat by auto.
-        rewrite mod_pow_pos_1_l.
-        rewrite Z.mod_1_l by lia.
-        rewrite Z.mul_1_l.
-        rewrite Z.rem_mod_nonneg by lia.
-        now rewrite mod_pow_pos_mod.
+    intros isprime ap0.
+    rewrite <- mod_inv_mod.
+    apply mod_mul_both_l with (mod_inv a p); auto.
+    rewrite mul_mod_inv by auto.
+    now rewrite Z.mul_comm, mul_mod_inv by auto.
   Qed.
-*)
 
-  Lemma mod_pow_exp a x p :
+  Lemma mod_pow_exp_mul a x x' p :
+    prime p ->
+    a mod p <> 0 ->
+    mod_pow a (x * x') p = mod_pow (mod_pow a x p) x' p.
+  Proof.
+    intros isprime ap0.
+    pose proof (prime_ge_2 _ isprime).
+    destruct x, x'; cbn;
+      repeat (
+          try rewrite Z.mod_1_l by lia;
+          try rewrite mod_pow_pos_1_l;
+          try rewrite mod_inv_1_l);
+      auto.
+    - apply mod_pow_pos_exp_mul.
+    - now rewrite mod_pow_pos_exp_mul.
+    - unfold mod_inv.
+      rewrite <- !mod_pow_pos_exp_mul.
+      rewrite <- Pos.mul_assoc.
+      now rewrite (Pos.mul_comm p1).
+    - unfold mod_inv.
+      rewrite <- !mod_pow_pos_exp_mul.
+      replace (p0 * (Z.to_pos (p - 2) * (p1 * Z.to_pos (p - 2))))%positive
+        with (p0 * p1 * Z.to_pos (p - 2) * Z.to_pos (p - 2))%positive
+        by lia.
+      rewrite !mod_pow_pos_exp_mul.
+      pose proof mod_inv_involutive.
+      unfold mod_inv in H0.
+      rewrite H0 by auto.
+      now rewrite mod_pow_pos_mod.
+  Qed.
+
+  Lemma mod_pow_exp_opp a x p :
+    prime p ->
+    a mod p <> 0 ->
+    mod_pow a (-x) p = mod_inv (mod_pow a x p) p.
+  Proof.
+    intros isprime ap0.
+    pose proof (prime_ge_2 _ isprime).
+    destruct x; auto.
+    - cbn.
+      rewrite mod_inv_mod_idemp.
+      now rewrite mod_inv_1_l.
+    - cbn.
+      rewrite mod_inv_involutive by auto.
+      now rewrite mod_pow_pos_mod.
+  Qed.
+
+  Lemma mod_pow_exp_mod a x p :
     prime p ->
     a mod p <> 0 ->
     mod_pow a (x mod (p - 1)) p = mod_pow a x p.
   Proof.
     intros isprime ap.
     pose proof (prime_ge_2 _ isprime).
-    pose proof (Z.mod_pos_bound x (p - 1) ltac:(lia)).
-    unfold mod_pow.
-    destruct (x <? 0) eqn:lt.
-    - apply Z.ltb_lt in lt.
-      destruct x; try lia.
-      cbn.
-      pose proof (Z.mod_pos_bound (Z.neg p0) (p - 1) ltac:(lia)).
-      destruct (Z.neg p0 mod (p - 1)) eqn:?; try lia.
-      + pose proof (Z.neg p0
     rewrite (Z.div_mod x (p - 1)) at 2 by lia.
-    rewrite !mod_pow_spec.
-    rewrite mod_pow_plus.
-    rewrite <- Z.add_mod_idemp_l by lia.
-    rewrite Z.mul_comm, Z.mod_mul by lia.
-    cbn.
-    destruct (x <? 0) eqn:lt.
-    - apply Z.ltb_lt in lt.
-      Search (Z.rem).
-Z.rem_bound_pos: forall a b : Z, 0 <= a -> 0 < b -> 0 <= Z.rem a b < b
-      rewrite Z.rem_
-    cbn.
-    rewrite Z.mod_small; cycle 1.
-    { Search (Z.rem _ _).
-      apply Z.rem_bound_pos.
-    rewrite mod_pow_spec by lia.
-    rewrite
-    rewrite Z.div_mod.
-    Search (_ ^ (_ + _)).
-    rewrite Z.pow_add_r.
-    unfold mod_pow.
-    destruct p; auto.
-    - pose proof (Z.mod_pos_bound x (Z.pos p - 1) ltac:(lia)).
-      destruct (x mod (Z.pos p - 1)) eqn:?; try lia.
-      + destruct x; try lia.
-        * rewrite <- mod_pow_pos_idemp by lia.
-          assert (Z.pos p0
-          replace (p0 with
-          assert (p0
-          replace p0
-      destruct (x mod (Z.pos p - 1)
+    rewrite mod_pow_exp_plus by auto.
+    rewrite mod_pow_exp_mul by auto.
+    rewrite mod_pow_fermat by auto.
+    rewrite mod_pow_1_l, !Z.mod_1_l by lia.
+    now rewrite Z.mul_1_l, mod_pow_mod.
+  Qed.
 
-
-    all: pose proof (Z.mod_pos_bound x (Z.pos p - 1)).
-
-    all:
-    rewrite mod_pow_pos_spec.
-
-  Lemma mod_pow_fermat_pos a p :
-    prime p ->
-    a mod p <> 0 ->
-    mod_pow a (p - 1) p = 1.
+  Definition Zp (p : Z) :
+    prime p -> BoardroomField Z.
   Proof.
-    intros isprime ap.
-    unfold mod_pow.
+    intros isprime.
     pose proof (prime_ge_2 _ isprime).
-    pose proof (mod_pow_pos_fermat _ _ isprime ap).
-    destruct p; try lia.
-    destruct (Z.pos p - 1) eqn:?; try lia.
-    assumption.
-  Qed.
+    refine
+      {|
+        elmeq a b := a mod p = b mod p;
+        zero := 0;
+        one := 1;
+        add a a' := (a + a') mod p;
+        mul a a' := (a * a') mod p;
+        opp a := p - a;
+        inv a := mod_inv a p;
+        pow a e := mod_pow a e p;
+        order := p;
+      |}.
+    - intros x y; apply Z.eq_dec.
+    - lia.
+    - constructor; auto.
+      now intros a a' a'' -> ->.
+    - intros a a' aeq b b' beq.
+      now rewrite Z.add_mod, aeq, beq, <- Z.add_mod by lia.
+    - intros a a' aeq b b' beq.
+      now rewrite Z.mul_mod, aeq, beq, <- Z.mul_mod by lia.
+    - intros a a' aeq.
+      now rewrite Zminus_mod, aeq, <- Zminus_mod.
+    - intros a a' aeq.
+      now rewrite <- mod_inv_mod_idemp, aeq, mod_inv_mod_idemp.
+    - intros a a' aeq e e' ->.
+      now rewrite <- !(mod_pow_mod_idemp a), aeq, !mod_pow_mod_idemp.
+    - intros a anp e e' eeq.
+      rewrite <- (mod_pow_exp_mod _ e), <- (mod_pow_exp_mod _ e') by auto.
+      now rewrite eeq.
+    - now rewrite Z.mod_1_l, Z.mod_0_l by lia.
+    - intros a b.
+      now rewrite Z.add_comm.
+    - intros a b c.
+      rewrite !Z.mod_mod by lia.
+      rewrite Z.add_mod_idemp_l, Z.add_mod_idemp_r by lia.
+      apply f_equal2; lia.
+    - intros a b.
+      now rewrite Z.mul_comm.
+    - intros a b c.
+      repeat (try rewrite Z.mul_mod_idemp_l; try rewrite Z.mul_mod_idemp_r); try lia.
+      now rewrite Z.mul_assoc.
+    - intros a.
+      now rewrite Z.mod_mod by lia.
+    - intros a.
+      now rewrite Z.mod_mod by lia.
+    - intros a.
+      rewrite Z.mod_mod by lia.
+      now rewrite Z.mul_1_l.
+    - intros a.
+      rewrite Z.mod_mod by lia.
+      replace (p - a + a) with p by lia.
+      rewrite Z.mod_same, Z.mod_0_l; lia.
+    - intros a anp.
+      now rewrite Z.mul_comm, mul_mod_inv by auto.
+    - intros a b c.
+      repeat (try rewrite Z.mul_mod_idemp_l;
+              try rewrite Z.mul_mod_idemp_r;
+              try rewrite Z.add_mod_idemp_l;
+              try rewrite Z.add_mod_idemp_r;
+              try rewrite Z.mod_mod); try lia.
+      apply f_equal2; lia.
+    - intros a anp.
+      cbn.
+      now rewrite Z.mod_1_l at 1 by lia.
+    - intros a.
+      now rewrite mod_pow_mod, mod_pow_1_r.
+    - intros a ap0.
+      rewrite (mod_pow_exp_opp _ 1) by auto.
+      rewrite mod_pow_1_r.
+      now rewrite mod_inv_mod_idemp.
+    - intros a e e' ap0.
+      now rewrite mod_pow_exp_plus by auto.
+    - auto.
+    - auto.
+  Defined.
+End Zp.
 
-  Lemma
-
-  (*
-  Lemma for_nonneg_exponent (P : Z -> Z -> Z -> Prop) p :
-    p >= 2 ->
-    (forall a, P a Z0 (mod_pow a Z0 p)) ->
-    (forall a x, P a (Z.pos x) (mod_pow a (Z.pos x) p)) ->
-    forall a x, P a x (mod_pow a x p).
-  Proof.
-    intros zero_case pos_case a x.
-    unfold mod_pow in *.
-    rewrite Z.quot_rem'
-    destruct (Z.eq_dec p 0) as [->|ne].
-    -
-    destruct x; auto.
-  Qed.
-*)
-
-
-
-Z.rem_mod: forall a b : Z, b <> 0 -> Z.rem a b = Z.sgn a * (Z.abs a mod Z.abs b)
-
-Section BigZp.
-  Section
+Module BigZp.
   Local Open Scope bigZ.
-  Fixpoint mod_pow_aux (a : bigZ) (x : positive) (m : bigZ) (r : bigZ) : bigZ :=
+  Fixpoint mod_pow_pos_aux (a : bigZ) (x : positive) (m : bigZ) (r : bigZ) : bigZ :=
     match x with
-    | x~0%positive => mod_pow_aux (BigZ.square a mod m) x m r
-    | x~1%positive => mod_pow_aux (BigZ.square a mod m) x m (r * a mod m)
+    | x~0%positive => mod_pow_pos_aux (BigZ.square a mod m) x m r
+    | x~1%positive => mod_pow_pos_aux (BigZ.square a mod m) x m (r * a mod m)
     | _ => r * a mod m
     end.
 
-  Definition mod_pow (a x p : bigZ) : bigZ :=
-    if p =? 0 then
-      0
-    else if x =? 0 then
-      a^0 mod p
-    else if 0 <? x then
-      mod_pow_aux a (Z.to_pos (BigZ.to_Z x)) p 1
-    else
-      mod_pow_aux
-        (mod_pow_aux a (Z.to_pos (BigZ.to_Z (-x))) p 1)
-        (Z.to_pos (BigZ.to_Z (p - 2)))
-        p 1.
+  Definition mod_pow_pos (a : bigZ) (x : positive) (m : bigZ) : bigZ :=
+    mod_pow_pos_aux a x m 1.
 
+  Definition mod_inv (a : bigZ) (p : bigZ) : bigZ :=
+    mod_pow_pos a (Z.to_pos (BigZ.to_Z (p - 2))) p.
 
-  Local Open Scope Z.
+  Definition mod_pow (a : bigZ) (x : Z) (p : bigZ) : bigZ :=
+    match x with
+    | Z0 => a ^ 0 mod p
+    | Zpos x => mod_pow_pos a x p
+    | Zneg x => mod_inv (mod_pow_pos a x p) p
+    end.
 
   Hint Rewrite BigZ.square_spec BigZ.spec_pow_pos : zsimpl.
   Hint Rewrite BigN.spec_of_pos : nsimpl.
@@ -2351,9 +1458,8 @@ Section BigZp.
   Qed.
 
   Instance mod_pow_aux_wd :
-    Proper (BigZ.eq ==> eq ==> BigZ.eq ==> BigZ.eq ==> BigZ.eq) mod_pow_aux.
+    Proper (BigZ.eq ==> eq ==> BigZ.eq ==> BigZ.eq ==> BigZ.eq) mod_pow_pos_aux.
   Proof.
-    (*intros a1 a2 elmeq ? x -> m1 m2 meq r1 r2 elmeq.*)
     intros a1 a2 elmeq ? x ->.
     revert a1 a2 elmeq.
     induction x; intros a1 a2 aeq m1 m2 meq r1 r2 req.
@@ -2376,8 +1482,8 @@ Section BigZp.
       reflexivity.
   Qed.
 
-  Lemma spec_mod_pow_aux a x p r :
-    [mod_pow_aux a x p r] = mod_pow_aux_Z [a] x [p] [r].
+  Lemma spec_mod_pow_pos_aux a x p r :
+    [mod_pow_pos_aux a x p r] = Zp.mod_pow_pos_aux [a] x [p] [r].
   Proof.
     revert a p r.
     induction x; intros a p r; cbn in *.
@@ -2387,109 +1493,38 @@ Section BigZp.
       now autorewrite with zsimpl.
     - now autorewrite with zsimpl.
   Qed.
+  Hint Rewrite spec_mod_pow_pos_aux : zsimpl.
 
-  Hint Rewrite spec_mod_pow_aux : zsimpl.
+  Lemma spec_mod_pow_pos a x p :
+    [mod_pow_pos a x p] = Zp.mod_pow_pos [a] x [p].
+  Proof. apply spec_mod_pow_pos_aux. Qed.
+  Hint Rewrite spec_mod_pow_pos : zsimpl.
+
+  Lemma spec_mod_inv a p :
+    [mod_inv a p] = Zp.mod_inv [a] [p].
+  Proof.
+    unfold mod_inv, Zp.mod_inv.
+    now autorewrite with zsimpl.
+  Qed.
+  Hint Rewrite spec_mod_inv : zsimpl.
 
   Lemma spec_mod_pow a x p :
-    [mod_pow a x p] = mod_pow_Z [a] [x] [p].
+    [mod_pow a x p] = Zp.mod_pow [a] x [p].
   Proof.
-    unfold mod_pow, mod_pow_Z.
-    autorewrite with zsimpl.
-    destruct (Z.eqb_spec [p] 0) as [->|ne]; auto; cbn.
-    rewrite (proj2 (Z.eqb_neq _ _) ne).
-    destruct (Z.compare_spec [x] [0]) as [->|?|?]; cbn in *.
-    - autorewrite with zsimpl.
-      destruct [p] eqn:eq; auto; congruence.
-    - rewrite (proj2 (Z.eqb_neq [x] 0) ltac:(lia)).
-      rewrite (proj2 (Z.ltb_ge 0 [x]) ltac:(lia)).
-      autorewrite with zsimpl.
-      destruct [x] eqn:?; try lia.
-      cbn.
-      destruct [p]; auto; congruence.
-    - rewrite (proj2 (Z.eqb_neq [x] 0) ltac:(lia)).
-      rewrite (proj2 (Z.ltb_lt 0 [x]) ltac:(lia)).
-      autorewrite with zsimpl.
-      destruct [x] eqn:?; try lia.
-      cbn.
-      destruct [p]; auto; congruence.
+    unfold mod_pow, Zp.mod_pow.
+    now destruct x; autorewrite with zsimpl.
   Qed.
-
   Hint Rewrite spec_mod_pow : zsimpl.
 
-  Local Open Scope bigZ.
-  Lemma mod_pow_spec a x p :
-    x >= 0 ->
-    mod_pow a x p == a^x mod p.
-  Proof.
-    intros xp.
-    unfold "==", "<=" in *; cbn in *.
-    autorewrite with zsimpl in *.
-    apply mod_pow_Z_spec.
-    lia.
-  Qed.
+  Hint Rewrite BigZ.spec_modulo : zsimpl.
 
-  Local Open Scope Z.
-  Local Open Scope bigZ.
-  Lemma mod_pow_mod_idemp a x p :
-    mod_pow (a mod p) x p == mod_pow a x p.
-  Proof.
-    unfold "==".
-    autorewrite with zsimpl.
-    now rewrite mod_pow_Z_mod_idemp.
-  Qed.
-
-  Lemma mod_inv_spec x m :
-    prime m ->
-    x mod m <> 0 ->
-    (x * mod_inv x m) mod m = 1.
-  Proof.
-    intros is_prime xnm.
-    pose proof (prime_ge_2 _ is_prime).
-    unfold mod_inv.
-    rewrite (mod_pow_spec x (m - 2) m).
-    rewrite Z.mul_mod_idemp_r by lia.
-    rewrite <- Z.pow_succ_r by lia.
-    replace (Z.succ (m - 2)) with (m - 1) by lia.
-    (* Use proof of Euler's theorem from Coqprime *)
-    rewrite <- (Euler.prime_phi_n_minus_1 _ is_prime).
-    apply phi_power_is_1; try lia.
-    apply rel_prime_sym.
-    apply prime_rel_prime; auto.
-    intros div.
-    pose proof (Zdivide_mod _ _ div).
-    tauto.
-  Qed.
-
-  Lemma mod_inv_mod_idemp (x m : Z) :
-    mod_inv (x mod m) m = mod_inv x m.
-  Proof.
-    unfold mod_inv.
-    rewrite 2!mod_pow_spec.
-    now rewrite Z_pow_mod_idemp.
-  Qed.
-
-  Lemma mod_inv_mul a b m :
-    mod_inv (a * b) m =
-    (mod_inv a m * mod_inv b m) mod m.
-  Proof.
-    unfold mod_inv.
-    now rewrite !mod_pow_spec, Z.pow_mul_l, Zmult_mod.
-  Qed.
-
-  Lemma mod_pow_exp_fermat a e p :
-    prime p ->
-    mod_pow a (e mod p - 1) p = mod_pow a e p.
-  Proof.
-    Search (_ * _ + _).
-
-  Local Open Scope Z.
-  Definition Zp_ffield (p : Z) :
-    prime p -> FField Z.
+  Definition BigZp (p : bigZ) :
+    prime [p] -> BoardroomField bigZ.
   Proof.
     intros isprime.
     pose proof (prime_ge_2 _ isprime).
     refine
-      {| elmeq a b := a mod p = b mod p;
+      {| elmeq a b := a mod p == b mod p;
          zero := 0;
          one := 1;
          add a a' := (a + a') mod p;
@@ -2497,59 +1532,69 @@ Section BigZp.
          opp a := p - a;
          inv a := mod_inv a p;
          pow a e := mod_pow a e p;
-         order := p;
-      |}.
+         order := BigZ.to_Z p;
+      |}; unfold "==".
     - intros x y.
       apply Z.eq_dec.
     - lia.
     - constructor; auto.
       now intros a a' a'' -> ->.
     - intros a a' aeq b b' beq.
+      autorewrite with zsimpl in *.
       now rewrite Z.add_mod, aeq, beq, <- Z.add_mod by lia.
     - intros a a' aeq b b' beq.
+      autorewrite with zsimpl in *.
       now rewrite Z.mul_mod, aeq, beq, <- Z.mul_mod by lia.
     - intros a a' aeq.
+      autorewrite with zsimpl in *.
       now rewrite Zminus_mod, aeq, <- Zminus_mod.
     - intros a a' aeq.
-      now rewrite <- mod_inv_mod_idemp, aeq, mod_inv_mod_idemp.
+      autorewrite with zsimpl in *.
+      now rewrite <- Zp.mod_inv_mod_idemp, aeq, Zp.mod_inv_mod_idemp.
     - intros a a' aeq e e' ->.
-      now rewrite <- !(mod_pow_mod_idemp a), aeq, !mod_pow_mod_idemp.
+      autorewrite with zsimpl in *.
+      now rewrite <- !(Zp.mod_pow_mod_idemp [a]), aeq, !Zp.mod_pow_mod_idemp.
     - intros a anp e e' eeq.
-      cbn in anp.
-
-      rewrite (proj2 (Z.eqb_neq _ _) anp).
+      autorewrite with zsimpl in *.
+      rewrite <- (Zp.mod_pow_exp_mod _ e), <- (Zp.mod_pow_exp_mod _ e') by auto.
       now rewrite eeq.
-    - now rewrite Z.mod_1_l, Z.mod_0_l by lia.
+    - autorewrite with zsimpl in *.
+      now rewrite Z.mod_1_l, Z.mod_0_l by lia.
     - intros a b.
-      now replace (a + b) with (b + a) by lia.
+      autorewrite with zsimpl in *.
+      now rewrite Z.add_comm.
     - intros a b c.
+      autorewrite with zsimpl in *.
       rewrite !Z.mod_mod by lia.
       rewrite Z.add_mod_idemp_l, Z.add_mod_idemp_r by lia.
       apply f_equal2; lia.
     - intros a b.
-      now replace (a * b) with (b * a) by lia.
+      autorewrite with zsimpl in *.
+      now rewrite Z.mul_comm.
     - intros a b c.
+      autorewrite with zsimpl in *.
       repeat (try rewrite Z.mul_mod_idemp_l; try rewrite Z.mul_mod_idemp_r); try lia.
-      now replace (a * (b * c)) with (a * b * c) by lia.
+      now rewrite Z.mul_assoc.
     - intros a.
+      autorewrite with zsimpl in *.
       now rewrite Z.mod_mod by lia.
     - intros a.
+      autorewrite with zsimpl in *.
       now rewrite Z.mod_mod by lia.
     - intros a.
+      autorewrite with zsimpl in *.
       rewrite Z.mod_mod by lia.
-      now replace (1 * a) with a by lia.
+      now rewrite Z.mul_1_l.
     - intros a.
+      autorewrite with zsimpl in *.
       rewrite Z.mod_mod by lia.
-      replace (p - a + a) with p by lia.
+      replace ([p] - [a] + [a])%Z with [p] by lia.
       rewrite Z.mod_same, Z.mod_0_l; lia.
     - intros a anp.
-      rewrite Z.mod_0_l, Z.mod_1_l in * by lia.
-      pose proof (mod_inv_spec _ _ isprime anp).
-      rewrite Z.mod_mod by lia.
-      now rewrite Z.mul_comm.
-    - intros a b anp bnp.
-      now rewrite mod_inv_mod_idemp, mod_inv_mul.
+      autorewrite with zsimpl in *.
+      now rewrite Z.mul_comm, Zp.mul_mod_inv by auto.
     - intros a b c.
+      autorewrite with zsimpl in *.
       repeat (try rewrite Z.mul_mod_idemp_l;
               try rewrite Z.mul_mod_idemp_r;
               try rewrite Z.add_mod_idemp_l;
@@ -2557,101 +1602,25 @@ Section BigZp.
               try rewrite Z.mod_mod); try lia.
       apply f_equal2; lia.
     - intros a anp.
+      autorewrite with zsimpl in *.
       cbn.
-      rewrite mod_pow_spec.
-      rewrite Z.pow_0_r.
-      now destruct (a mod p =? 0);
-        rewrite Z.mod_mod by lia.
+      now rewrite Z.mod_1_l at 1 by lia.
     - intros a.
-      rewrite !mod_pow_spec.
-      destruct (Z.eq_dec p 2) as [->|?].
-      + destruct (Z.eq_dec (a mod 2) 0) as [eq|neq].
-        * rewrite eq.
-          cbn.
-          now rewrite Z.mul_1_r, eq.
-        * rewrite (proj2 (Z.eqb_neq _ _) neq).
-          cbn.
-          pose proof (Z.mod_pos_bound a 2 ltac:(lia)).
-          lia.
-      + rewrite Z.mod_1_l by lia.
-        rewrite Z.pow_1_r.
-        destruct (a mod p =? 0); apply Z.mod_mod; lia.
+      autorewrite with zsimpl in *.
+      now rewrite Zp.mod_pow_mod, Zp.mod_pow_1_r.
     - intros a ap0.
-      cbn in ap0.
-      rewrite (proj2 (Z.eqb_neq _ _) ap0).
-      unfold mod_inv.
-      destruct (Z.eq_dec p 2) as [->|?]; auto.
-      rewrite (Z_mod_nz_opp_full 1) by (rewrite Z.mod_1_l by lia; lia).
-      rewrite Z.mod_1_l by lia.
-      now replace (p - 1 - 1) with (p - 2) by lia.
+      autorewrite with zsimpl in *.
+      rewrite (Zp.mod_pow_exp_opp _ 1) by auto.
+      rewrite Zp.mod_pow_1_r.
+      now rewrite Zp.mod_inv_mod_idemp.
     - intros a e e' ap0.
-      cbn in ap0.
-      rewrite (proj2 (Z.eqb_neq _ _) ap0).
-      rewrite Z.add_mod by lia.
-      rewrite !mod_pow_spec.
-      rewrite !Z.mod_mod by lia.
-      destruct (Z.eq_dec (a mod p) 0) as [eq|ne].
-      + rewrite eq.
-        cbn.
-        rewrite !mod_pow_spec.
-        Search (_ ^ (_ + _)).
-        rewrite Z.pow_add_r.
-        rewrite
-    - intros a e anp.
-      rewrite mod_pow_spec.
-      cbn.
-      assert (apprime : forall a, a mod p <> 0 -> rel_prime a p).
-      {
-        clear -isprime.
-        intros a amodp.
-        apply rel_prime_sym.
-        apply prime_rel_prime; auto.
-        intros div. apply Zdivide_mod in div.
-        congruence.
-      }
-
-      assert (1 < p) as ltp by lia.
-      assert (gpow_mod :
-                forall a e,
-                  a mod p <> 0 ->
-                  0 <= e ->
-                  a ^ e mod p = gpow (a mod p) (ZPGroup p ltp) e).
-      {
-        clear -isprime apprime.
-        intros a e ap0 ege.
-        apply Zpower_mod_is_gpow; auto.
-      }
-
-      assert (0 <= e mod (p - 1))
-        by (pose proof (Z.mod_pos_bound e (p - 1) ltac:(lia)); lia).
-      rewrite gpow_mod; auto.
-      assert (in_zpstar: forall a, a mod p <> 0 <-> List.In (a mod p)
-                                                            (FGroup.s (ZPGroup p ltp))).
-      {
-        clear -isprime apprime.
-        intros a.
-        split.
-        - intros ap0.
-          apply in_mod_ZPGroup.
-          auto.
-        - intros isin.
-          cbn in *.
-          pose proof (IGroup.isupport_is_inv_true _ _ _ _ _ _ isin).
-          rewrite rel_prime_is_inv in H by lia.
-          destruct (rel_prime_dec (a mod p) p); try congruence.
-          apply Zrel_prime_neq_mod_0; [lia|].
-          apply rel_prime_mod_rev; auto; lia.
-      }
-
-      apply in_zpstar.
-      rewrite <- gpow_mod; auto.
-      rewrite Z.mod_mod by lia.
-      rewrite gpow_mod; auto.
-      apply gpow_in.
-      now apply in_zpstar.
+      autorewrite with zsimpl in *.
+      now rewrite Zp.mod_pow_exp_plus by auto.
+    - intros a e ap0.
+      autorewrite with zsimpl in *.
+      auto.
+    - intros a ap0.
+      autorewrite with zsimpl in *.
+      auto.
   Defined.
-
-End Zp.
-
-Section WithZp.
-End WithZp.
+End BigZp.
